half of kleili proof

Move_SEC.thy
@@ -2,25 +2,157 @@ theory Move_SEC
   imports Move CRDT.Network
 begin
 
-definition interp_op' :: \<open>('a::{linorder}, 'b) operation \<Rightarrow> ('a, 'b) state \<rightharpoonup> ('a, 'b) state\<close> where
-  \<open>interp_op' x s \<equiv> Some (interp_op x s)\<close>
+definition interp_op' :: \<open>('t::{linorder}, 'n, 'm) operation \<Rightarrow> ('t, 'n, 'm) state \<rightharpoonup> ('t, 'n, 'm) state\<close> where
+  \<open>interp_op' x s \<equiv> case s of (log, tree) \<Rightarrow>
+    if unique_parent tree \<and> distinct (map log_time log @ [move_time x]) then
+      Some (interp_op x s)
+    else None\<close>
 
-fun valid_move_opers :: "('b, 'c) state \<Rightarrow> 'b \<times> ('b, 'c) operation \<Rightarrow> bool" where
-  \<open>valid_move_opers S (i, Move t p c) = (t = i)\<close>
+fun valid_move_opers :: "('t, 'n, 'm) state \<Rightarrow> 't \<times>('t, 'n, 'm) operation \<Rightarrow> bool" where
+  \<open>valid_move_opers S (i, Move t _ _ _) = (t = i)\<close>
 
 locale move = network_with_constrained_ops _ "interp_op'" "([], {})" valid_move_opers
 begin
 
+
+lemma kleisli_interp_op' [iff]:
+  shows \<open>interp_op' (x :: ('t :: {linorder}, 'n, 'm) operation) \<rhd> interp_op' y = interp_op' y \<rhd> interp_op' x\<close>
+proof (unfold kleisli_def, rule ext, clarify)
+  fix log :: \<open>('t, 'n, 'm) log_op list\<close> and tree :: \<open>('n \<times> 'm \<times> 'n) set\<close>
+  { assume \<open>unique_parent tree\<close> \<open>distinct (map log_time log @ [move_time x])\<close> \<open>distinct (map log_time log @ [move_time y])\<close>
+    have \<open>interp_op' x (log, tree) \<bind> interp_op' y = interp_op' y (log, tree) \<bind> interp_op' x\<close>
+      sorry
+  }
+  moreover {
+    assume *: \<open>unique_parent tree\<close> \<open>\<not> distinct (map log_time log @ [move_time x])\<close> \<open>distinct (map log_time log @ [move_time y])\<close>
+    then have **: \<open>move_time x \<in> set (map log_time log)\<close>
+      by auto 
+    obtain log1 tree1 where \<open>interp_op y (log, tree) = (log1, tree1)\<close>
+      using * by (clarsimp simp: interp_op'_def)  (metis surj_pair)
+    moreover hence \<open> set (map log_time log1) = {move_time y} \<union> set (map log_time log)\<close>
+      using * by (cases y) (rule interp_op_timestampI2; force)
+    hence \<open>move_time x \<in> set (map log_time log1)\<close>
+      using ** by blast
+    moreover hence \<open>\<not> distinct (map log_time log1 @ [move_time x])\<close>
+      by simp
+    ultimately have \<open>interp_op' x (log, tree) \<bind> interp_op' y = interp_op' y (log, tree) \<bind> interp_op' x\<close>
+      using * by (clarsimp simp: interp_op'_def)
+  }
+  moreover {
+    assume *: \<open>unique_parent tree\<close> \<open>distinct (map log_time log @ [move_time x])\<close> \<open>\<not> distinct (map log_time log @ [move_time y])\<close>
+    then have **: \<open>move_time y \<in> set (map log_time log)\<close>
+      by auto 
+    obtain log1 tree1 where \<open>interp_op x (log, tree) = (log1, tree1)\<close>
+      using * by (clarsimp simp: interp_op'_def)  (metis surj_pair)
+    moreover hence \<open> set (map log_time log1) = {move_time x} \<union> set (map log_time log)\<close>
+      using * by (cases x) (rule interp_op_timestampI2; force)
+    hence \<open>move_time y \<in> set (map log_time log1)\<close>
+      using ** by blast
+    moreover hence \<open>\<not> distinct (map log_time log1 @ [move_time y])\<close>
+      by simp
+    ultimately have \<open>interp_op' x (log, tree) \<bind> interp_op' y = interp_op' y (log, tree) \<bind> interp_op' x\<close>
+      using * by (clarsimp simp: interp_op'_def)
+  }
+  ultimately show \<open>interp_op' x (log, tree) \<bind> interp_op' y = interp_op' y (log, tree) \<bind> interp_op' x\<close>
+    by (clarsimp simp: interp_op'_def)
+
+qed
+(*
+  apply(rule ext)
+  apply clarify
+  apply (case_tac \<open>unique_parent b \<and> distinct (map log_time a)\<close>)
+   prefer 2
+   apply force
+  apply (case_tac \<open>distinct (map log_time a @ [move_time x, move_time y])\<close>)
+   apply clarify
+   apply (case_tac \<open>interp_op x (a, b)\<close>)
+   apply (case_tac \<open>interp_op y (a, b)\<close>)
+   apply (subgoal_tac \<open>unique_parent ba \<and> unique_parent bb\<close>)
+  prefer 2
+  using interp_op_unique_parent apply blast
+  apply clarsimp
+  apply (subgoal_tac \<open>distinct (map log_time aa) \<and>
+                      distinct (map log_time ab)\<close>)
+    prefer 2
+    apply (rule conjI)
+     apply (cases x)
+     apply clarsimp
+      apply (rule interp_op_timestampI1)
+       prefer 2
+       apply assumption
+     apply force
+     apply (cases y)
+     apply clarsimp
+      apply (rule interp_op_timestampI1)
+       prefer 2
+       apply assumption
+    apply force
+   apply clarsimp
+   apply (case_tac \<open>move_time x \<notin> log_time ` set ab \<and> move_time y \<notin> log_time ` set aa\<close>)
+    apply clarsimp
+    apply (cases x, cases y)
+  apply clarsimp
+    apply (rule interp_op_commute2I)
+       apply force
+      apply force
+     apply force
+    apply force
+  
+
+*)
+
+(*
 lemma timestamps_distinct:
   assumes \<open>xs prefix of i\<close>
   and \<open>ops = node_deliver_messages xs\<close>
 shows \<open>distinct (map (move_time \<circ> snd) ops)\<close>
-  sorry
+  sorry*)
 
 lemma kleisli_interp_op' [iff]:
-  shows \<open>interp_op' x \<rhd> interp_op' y = interp_op' y \<rhd> interp_op' x\<close>
-  apply(clarsimp simp add: interp_op'_def kleisli_def)
+  shows \<open>interp_op' x \<rhd> interp_op' y = interp_op' y \<rhd> interp_op' x\<close>  
+  apply(unfold interp_op'_def kleisli_def)
   apply(rule ext)
+  apply clarify
+  apply (case_tac \<open>unique_parent b \<and> distinct (map log_time a)\<close>)
+   prefer 2
+   apply force
+  apply (case_tac \<open>distinct (map log_time a @ [move_time x, move_time y])\<close>)
+   apply clarify
+   apply (case_tac \<open>interp_op x (a, b)\<close>)
+   apply (case_tac \<open>interp_op y (a, b)\<close>)
+   apply (subgoal_tac \<open>unique_parent ba \<and> unique_parent bb\<close>)
+  prefer 2
+  using interp_op_unique_parent apply blast
+  apply clarsimp
+  apply (subgoal_tac \<open>distinct (map log_time aa) \<and>
+                      distinct (map log_time ab)\<close>)
+    prefer 2
+    apply (rule conjI)
+     apply (cases x)
+     apply clarsimp
+      apply (rule interp_op_timestampI1)
+       prefer 2
+       apply assumption
+     apply force
+     apply (cases y)
+     apply clarsimp
+      apply (rule interp_op_timestampI1)
+       prefer 2
+       apply assumption
+    apply force
+   apply clarsimp
+   apply (case_tac \<open>move_time x \<notin> log_time ` set ab \<and> move_time y \<notin> log_time ` set aa\<close>)
+    apply clarsimp
+    apply (cases x, cases y)
+  apply clarsimp
+    apply (rule interp_op_commute2I)
+       apply force
+      apply force
+     apply force
+    apply force
+  
+
+
   
 
 lemma concurrent_operations_commute:
@@ -29,6 +161,8 @@ lemma concurrent_operations_commute:
   using assms
   apply(clarsimp simp add: hb.concurrent_ops_commute_def)
   apply(unfold interp_msg_def; simp)
+  prefer 2
+  
   done
 
 sublocale sec: strong_eventual_consistency weak_hb hb interp_msg
